common/ghash.ml
@@ -1,0 +1,177 @@
+(* ========================================================================= *)
+(* GHASH polynomial both via machine words and as an element of GF(2)[X].    *)
+(* ========================================================================= *)
+
+needs "common/misc.ml";;
+needs "Library/rabin_test.ml";;
+
+(* ------------------------------------------------------------------------- *)
+(* Some basics for univariate polynomials to be less tiresome.               *)
+(* The library theory of polynomials has some cruft for arbitrary monomials. *)
+(* ------------------------------------------------------------------------- *)
+
+let coeff = define
+ `coeff:num->1->num = \d v. d`;;
+
+let POLY_MUL_UNIVARIATE = prove
+ (`!r (p:(1->num)->R) q.
+      poly_mul r p q =
+      \m. ring_sum r (0..m one)
+              (\i. ring_mul r (p(coeff i)) (q(coeff(m one - i))))`,
+  REPEAT GEN_TAC THEN REWRITE_TAC[poly_mul; coeff] THEN
+  GEN_REWRITE_TAC I [FUN_EQ_THM] THEN
+  GEN_REWRITE_TAC I [FORALL_FUN_FROM_1] THEN
+  X_GEN_TAC `k:num` THEN REWRITE_TAC[] THEN
+  MATCH_MP_TAC RING_SUM_EQ_GENERAL_INVERSES THEN
+  EXISTS_TAC `\mm. (FST:(1->num)#(1->num)->1->num) mm one` THEN
+  EXISTS_TAC `\i. (\v:1. i),(\v:1. k - i)` THEN
+  REWRITE_TAC[FORALL_IN_GSPEC; IN_ELIM_PAIR_THM] THEN
+  REWRITE_TAC[FORALL_FUN_FROM_1; coeff; monomial_mul] THEN
+  REWRITE_TAC[MESON[] `(\x:1. a) = (\x. b) <=> a = b`] THEN
+  REWRITE_TAC[IN_NUMSEG; LE_0] THEN
+  SIMP_TAC[ARITH_RULE `i + j:num = k <=> i <= k /\ j = k - i`]);;
+
+(* ------------------------------------------------------------------------- *)
+(* A lemma for mapping between integer and boolean points of view            *)
+(* ------------------------------------------------------------------------- *)
+
+let BITVAL_RING_SUM_BOOL_RING = prove
+ (`!f (s:K->bool).
+        FINITE s
+        ==> bitval(ring_sum bool_ring s f) = nsum s (bitval o f) MOD 2`,
+  GEN_TAC THEN ONCE_REWRITE_TAC[EQ_SYM_EQ] THEN
+  MATCH_MP_TAC FINITE_INDUCT_STRONG THEN
+  SIMP_TAC[NSUM_CLAUSES; RING_SUM_CLAUSES; BOOL_RING; IN_UNIV] THEN
+  REWRITE_TAC[BITVAL_CLAUSES] THEN CONV_TAC NUM_REDUCE_CONV THEN
+  ONCE_REWRITE_TAC[GSYM MOD_ADD_MOD] THEN
+  MAP_EVERY X_GEN_TAC [`a:K`; `s:K->bool`] THEN STRIP_TAC THEN
+  ASM_REWRITE_TAC[BITVAL_NOT; BITVAL_IFF; BITVAL_CLAUSES] THEN
+  REWRITE_TAC[o_THM; bitval] THEN
+  REPEAT(COND_CASES_TAC THEN ASM_REWRITE_TAC[]) THEN
+  CONV_TAC NUM_REDUCE_CONV);;
+
+(* ------------------------------------------------------------------------- *)
+(* Correspondence between binary polynomials and machine words.              *)
+(* Polynomials are members of `poly_ring bool_ring (:1)` = GF(2)[X].         *)
+(* They are mapped to and from machine words of length N, type `:N word`.    *)
+(* ------------------------------------------------------------------------- *)
+
+let bool_poly = define
+ `bool_poly = poly_ring bool_ring (:1)`;;
+
+let word_of_poly = define
+ `(word_of_poly:((1->num)->bool)->N word) p = word_of_bits {i | p(coeff i)}`;;
+
+let poly_of_word = define
+ `(poly_of_word:N word->(1->num)->bool) w = \m. bit (m one) w`;;
+
+let BOOL_POLY_OF_WORD = prove
+ (`!w:N word. poly_of_word w IN ring_carrier bool_poly`,
+  REWRITE_TAC[bool_poly; POLY_RING; ring_polynomial; ring_powerseries;
+              IN_ELIM_THM; BOOL_RING; SUBSET_UNIV; IN_UNIV] THEN
+  REWRITE_TAC[FINITE_MONOMIAL_VARS_1; INFINITE] THEN
+  REWRITE_TAC[poly_of_word] THEN GEN_TAC THEN
+  MATCH_MP_TAC FINITE_SUBSET THEN
+  EXISTS_TAC `IMAGE coeff {i | i < dimindex(:N)}` THEN
+  SIMP_TAC[FINITE_IMAGE; FINITE_NUMSEG_LT; SUBSET; IN_ELIM_THM] THEN
+  REWRITE_TAC[FORALL_FUN_FROM_1; IN_IMAGE; IN_ELIM_THM; coeff] THEN
+  MESON_TAC[BIT_TRIVIAL; NOT_LE]);;
+
+let POLY_DEG_POLY_OF_WORD = prove
+ (`!w:N word. poly_deg bool_ring (poly_of_word w) < dimindex(:N)`,
+  GEN_TAC THEN
+  SIMP_TAC[DIMINDEX_NONZERO; ARITH_RULE
+   `~(n = 0) ==> (x < n <=> x <= n - 1)`] THEN
+  MATCH_MP_TAC POLY_DEG_LE THEN
+  REWRITE_TAC[RING_POLYNOMIAL; BOOL_POLY_OF_WORD; GSYM bool_poly] THEN
+  REWRITE_TAC[FORALL_FUN_FROM_1; BOOL_RING; MONOMIAL_DEG_UNIVARIATE] THEN
+  REWRITE_TAC[poly_of_word; coeff] THEN
+  ONCE_REWRITE_TAC[BIT_GUARD] THEN ARITH_TAC);;
+
+let WORD_OF_POLY_OF_WORD = prove
+ (`!w:N word. word_of_poly (poly_of_word w) = w`,
+  GEN_TAC THEN REWRITE_TAC[word_of_poly; poly_of_word] THEN
+  GEN_REWRITE_TAC I [WORD_EQ_BITS_ALT] THEN
+  SIMP_TAC[BIT_WORD_OF_BITS; coeff; IN_ELIM_THM]);;
+
+let WORD_OF_POLY_OF_WORD_GEN = prove
+ (`!w:N word. word_of_poly (poly_of_word w):M word = word_zx w`,
+  GEN_TAC THEN REWRITE_TAC[word_of_poly; poly_of_word] THEN
+  GEN_REWRITE_TAC I [WORD_EQ_BITS_ALT] THEN
+  SIMP_TAC[BIT_WORD_OF_BITS; BIT_WORD_ZX; coeff; IN_ELIM_THM]);;
+
+let POLY_OF_WORD_OF_POLY = prove
+ (`!p. p IN ring_carrier bool_poly /\
+       poly_deg bool_ring p < dimindex(:N)
+       ==> poly_of_word (word_of_poly p:N word) = p`,
+  REWRITE_TAC[bool_poly; GSYM RING_POLYNOMIAL] THEN
+  REPEAT STRIP_TAC THEN
+  FIRST_X_ASSUM(MP_TAC o SPEC `dimindex(:N)` o MATCH_MP POLY_DEG_GE_EQ) THEN
+  ASM_REWRITE_TAC[GSYM NOT_LT; DE_MORGAN_THM; NOT_EXISTS_THM] THEN
+  DISCH_THEN(MP_TAC o CONJUNCT2) THEN
+  GEN_REWRITE_TAC RAND_CONV [FUN_EQ_THM] THEN
+  REWRITE_TAC[FORALL_FUN_FROM_1; word_of_poly; poly_of_word] THEN
+  REWRITE_TAC[BIT_WORD_OF_BITS; coeff; BOOL_RING; MONOMIAL_DEG_UNIVARIATE] THEN
+  SET_TAC[]);;
+
+let POLY_OF_WORD_OF_POLY_EQ = prove
+ (`!p. p IN ring_carrier bool_poly
+       ==> (poly_of_word (word_of_poly p:N word) = p <=>
+            poly_deg bool_ring p < dimindex(:N))`,
+  MESON_TAC[POLY_OF_WORD_OF_POLY; POLY_DEG_POLY_OF_WORD]);;
+
+(* ------------------------------------------------------------------------- *)
+(* XOR and PMUL correspond to addition and multiplication of polynomials.    *)
+(* ------------------------------------------------------------------------- *)
+
+let WORD_XOR_POLY = prove
+ (`!x y:N word.
+        word_xor x y =
+        word_of_poly (ring_add bool_poly (poly_of_word x) (poly_of_word y))`,
+  REPEAT GEN_TAC THEN
+  GEN_REWRITE_TAC I [WORD_EQ_BITS_ALT] THEN
+  X_GEN_TAC `i:num` THEN DISCH_TAC THEN
+  REWRITE_TAC[word_of_poly; bool_poly; POLY_RING; BOOL_RING; poly_add] THEN
+  REWRITE_TAC[BIT_WORD_OF_BITS; IN_ELIM_THM; BIT_WORD_XOR] THEN
+  REWRITE_TAC[poly_of_word; coeff]);;
+
+let POLY_OF_WORD_XOR = prove
+ (`!(x:N word) (y:N word).
+        poly_of_word(word_xor x y) =
+        ring_add bool_poly (poly_of_word x) (poly_of_word y)`,
+  REPEAT GEN_TAC THEN REWRITE_TAC[WORD_XOR_POLY] THEN
+  MATCH_MP_TAC POLY_OF_WORD_OF_POLY THEN
+  SIMP_TAC[RING_ADD; BOOL_POLY_OF_WORD] THEN
+  REWRITE_TAC[bool_poly; POLY_RING] THEN
+  W(MP_TAC o PART_MATCH (lhand o rand) POLY_DEG_ADD_LE o lhand o snd) THEN
+  REWRITE_TAC[RING_POLYNOMIAL; BOOL_POLY_OF_WORD; GSYM bool_poly] THEN
+  MATCH_MP_TAC(REWRITE_RULE[IMP_CONJ_ALT] LET_TRANS) THEN
+  MATCH_MP_TAC(ARITH_RULE `x < n /\ y < n ==> MAX x y < n`) THEN
+  REWRITE_TAC[POLY_DEG_POLY_OF_WORD]);;
+
+let WORD_PMUL_POLY = prove
+ (`!x y. (word_pmul:M word->N word->P word) x y =
+         word_of_poly (ring_mul bool_poly (poly_of_word x) (poly_of_word y))`,
+  REPEAT GEN_TAC THEN
+  GEN_REWRITE_TAC I [WORD_EQ_BITS_ALT] THEN
+  X_GEN_TAC `i:num` THEN DISCH_TAC THEN
+  ASM_REWRITE_TAC[GSYM EQ_BITVAL; BITVAL_BIT_WORD_PMUL] THEN
+  REWRITE_TAC[word_of_poly; bool_poly; POLY_RING] THEN
+  ASM_REWRITE_TAC[POLY_MUL_UNIVARIATE; BIT_WORD_OF_BITS; IN_ELIM_THM] THEN
+  REWRITE_TAC[coeff; BOOL_RING] THEN
+  SIMP_TAC[BITVAL_RING_SUM_BOOL_RING; FINITE_NUMSEG] THEN
+  REWRITE_TAC[o_DEF; BITVAL_AND; poly_of_word]);;
+
+let POLY_OF_WORD_PMUL_2N = prove
+ (`!(x:N word) (y:N word).
+        poly_of_word(word_pmul x y:((N)tybit0)word) =
+        ring_mul bool_poly (poly_of_word x) (poly_of_word y)`,
+  REPEAT GEN_TAC THEN REWRITE_TAC[WORD_PMUL_POLY] THEN
+  MATCH_MP_TAC POLY_OF_WORD_OF_POLY THEN
+  SIMP_TAC[RING_MUL; BOOL_POLY_OF_WORD; DIMINDEX_TYBIT0] THEN
+  REWRITE_TAC[bool_poly; POLY_RING] THEN
+  W(MP_TAC o PART_MATCH (lhand o rand) POLY_DEG_MUL_LE o lhand o snd) THEN
+  REWRITE_TAC[RING_POLYNOMIAL; BOOL_POLY_OF_WORD; GSYM bool_poly] THEN
+  MATCH_MP_TAC(REWRITE_RULE[IMP_CONJ_ALT] LET_TRANS) THEN
+  MATCH_MP_TAC(ARITH_RULE `x < n /\ y < n ==> x + y < 2 * n`) THEN
+  REWRITE_TAC[POLY_DEG_POLY_OF_WORD]);;
